case_study/lean/Base/Small_Step.lean
@@ -1,0 +1,244 @@
+import Definitions.Com
+import Base.Big_Step
+
+theorem small_step_deterministic : (cs ->> cs') -> (cs ->> cs'') -> (cs'' = cs') := by
+  intros h1 h2
+  induction h1 generalizing cs'' with
+    | var_assign x a s=> 
+      cases h2
+      rfl
+    | seq_1 c2 s => 
+      cases h2 with
+        | seq_1 => rfl
+        | seq_2 _ _ _ _ _ h => cases h
+    | seq_2 c1 c1' c2 s s' h ih => 
+      cases h2 with
+        | seq_1 => cases h
+        | seq_2 _ c2' _ _ s'' h' =>
+          have conf_eq: ((c1', s') = (c2', s'')) := by
+            symm; apply ih; assumption
+          rcases conf_eq
+          rfl
+    | if_true b c1 c2 s cond =>
+      cases h2 with
+        | if_true => rfl
+        | if_false _ _ _ _ cond' =>
+          rw [cond] at cond'
+          trivial
+    | if_false b c1 c2 s cond =>
+      cases h2 with
+        | if_true _ _ _ _ cond' =>
+          rw [cond'] at cond
+          trivial
+        | if_false _ _ _ _ cond' => rfl
+    | while_loop b c s =>
+      cases h2; rfl
+
+
+theorem small_seq_congr : ((c_1, s_1) ->* (c, s_2)) -> (c_1;;c_2, s_1) ->* (c;;c_2, s_2) := by
+  intros h
+  generalize rn : (c_1, s_1) = p1
+  generalize rn' : (c, s_2) = p2
+  rw [rn, rn'] at h
+  induction h generalizing c c_1 s_1 c_2 s_2 with
+    | refl => cases rn; cases rn'; apply RTC.refl
+    | step cs cs' ht hh ih =>
+      cases rn; cases rn'
+      rcases cs with ⟨c_1', s_1'⟩ 
+      have h: (RTC SmallStep (c_1';;c_2, s_1') (c;;c_2, s_2)) := by
+        apply ih <;> rfl
+
+      have h': (RTC SmallStep (c_1;;c_2, s_1) (c_1';;c_2, s_1')) := by
+        apply RTC.step
+        apply SmallStep.seq_2
+        assumption
+        apply RTC.refl
+
+      apply RTC_trans <;> assumption      
+
+
+theorem big_imp_small : (cs ==> t) -> (cs ->* (SKIP, t)) := by
+  intro h
+  induction h with
+    | skip s =>
+      apply RTC.refl
+    | assign =>
+      apply RTC_single
+      apply SmallStep.var_assign
+    | seq c1 c2 s t u h1 h2 ih ih' =>
+      have h_mid_1 : ((c1;;c2, s) ->* (SKIP;;c2, t)) := by
+        apply small_seq_congr
+        assumption
+      have h_mid_2 : ((SKIP;;c2, t) ->* (c2, t)) := by
+        apply RTC_single
+        apply SmallStep.seq_1
+      repeat (apply RTC_trans; assumption)
+      apply RTC.refl
+    | if_true b c c' s t hcond hb ih =>
+      have h: (RTC SmallStep (IF b THEN c ELSE c', s) (c, s)) := by
+        apply RTC_single
+        apply SmallStep.if_true
+        assumption
+      apply RTC_trans <;> assumption
+    | if_false b c c' s t hcond hb ih =>
+      have h: (RTC SmallStep (IF b THEN c ELSE c', s) (c', s)) := by
+        apply RTC_single
+        apply SmallStep.if_false
+        assumption
+      apply RTC_trans <;> assumption
+    | while_false cond d s' hcond => {
+      apply (RTC.step (IF cond THEN d;;WHILE cond DO d ELSE SKIP, s'))
+      apply SmallStep.while_loop
+      apply RTC_single
+      apply SmallStep.if_false
+      assumption
+    }
+    | while_true cond d s' t' u hcond hb hr ih_c ih_r => {
+      have h1: (RTC SmallStep (WHILE cond DO d, s') (d;;WHILE cond DO d, s')) := by
+        have h2: (RTC SmallStep (WHILE cond DO d, s') (IF cond THEN d;;WHILE cond DO d ELSE SKIP, s')) := by
+          apply RTC_single
+          apply SmallStep.while_loop
+        apply RTC_trans
+        assumption
+        apply RTC_single
+        apply SmallStep.if_true
+        assumption
+
+      have h3: (RTC SmallStep (d;;WHILE cond DO d, s') (SKIP;;WHILE cond DO d, t') ) := by
+        apply small_seq_congr
+        assumption
+
+      have h4: (RTC SmallStep (SKIP;;WHILE cond DO d, t') (WHILE cond DO d, t') ) := by
+        apply RTC_single
+        apply SmallStep.seq_1
+
+      repeat (apply RTC_trans; assumption)
+      apply RTC.refl
+    }
+
+theorem step_sem_imp : (cs ->> cs') -> (cs' ==> t) -> (cs ==> t) := by
+  intros h h'
+  induction h generalizing t with
+    | var_assign =>
+      cases h'
+      apply BigStep.assign
+    | seq_1 =>
+      apply BigStep.seq
+      apply BigStep.skip
+      assumption
+    | seq_2 c1 c1' c2 s s' h'' ih =>
+      cases h' with
+        | seq _ _ _ t' _ hl hr =>
+          apply BigStep.seq
+          apply ih <;>
+          assumption
+          assumption
+    | if_true =>
+      apply BigStep.if_true <;>
+      assumption
+    | if_false => 
+      apply BigStep.if_false <;>
+      assumption
+    | while_loop =>
+      rw [unfold_while]
+      assumption
+
+theorem small_imp_big : (cs ->* (SKIP, t)) -> (cs ==> t) := by
+  intro h
+  generalize rn : (SKIP, t) = p
+  rw [rn] at h
+  induction h generalizing t with
+    | refl =>
+      cases rn
+      apply BigStep.skip
+    | step cs' cs'' hh ht ih =>
+      rcases cs' with ⟨c_1', s_1'⟩ 
+      cases rn
+      simp at ih
+      apply step_sem_imp <;>
+      assumption
+
+
+theorem small_big_eq : ((c, s) ==> t) <-> ((c, s) ->* (SKIP, t) ) := by
+  constructor
+  intro; apply big_imp_small; assumption
+  intro; apply small_imp_big; assumption
+
+theorem small_final : final (c, s) <-> (c = SKIP) := by
+  constructor
+  {
+    intro h
+    induction c with
+      | skip =>
+        rfl
+      | assign var val =>
+        exfalso
+        apply h
+        exists (SKIP, s[var ↦ (aeval val s)])
+        apply SmallStep.var_assign
+      | seq c c' ih ih' =>
+        exfalso
+        apply h
+        by_cases h'': (final (c, s))
+        have hc : (c = SKIP) := by
+          apply ih; assumption
+        cases hc
+        exists (c', s)
+        apply SmallStep.seq_1
+        simp [final] at h''
+        cases h'' with | intro d h''
+        cases h'' with | intro t h''
+        exists (d;;c', t)
+        apply SmallStep.seq_2
+        assumption
+      | ite cond ci ce ih ih' =>
+        exfalso
+        apply h
+        by_cases hcond:(beval cond s = true)
+        exists (ci, s)
+        apply SmallStep.if_true
+        assumption
+        exists (ce, s)
+        apply SmallStep.if_false
+        assumption
+      | «while» cond loop ih=>
+        exfalso
+        apply h
+        exists (IF cond THEN loop ;; WHILE cond DO loop ELSE SKIP, s)
+        apply SmallStep.while_loop
+  }
+  {
+    intro h; cases h
+    unfold final
+    intros cs h'
+    cases h' with | intro cs' h'
+    simp [cs] at h'
+    cases h'
+  }
+
+theorem big_step_small_step_termination : (exists t, cs ==> t) <-> (exists cs', cs ->* cs' ∧ final cs') := by
+  constructor
+  {
+    intro h
+    cases h with | intro t h
+    exists (SKIP, t)
+    constructor
+    rw [<- small_big_eq]
+    assumption
+    rw [small_final]
+  }
+  {
+    intro h
+    cases h with | intro cs' h
+    rcases h with ⟨h, h'⟩ 
+    rcases cs with ⟨c, s⟩ 
+    rcases cs' with ⟨c', t⟩ 
+    exists t
+    rw [small_big_eq]
+    have hc' : (c' = SKIP) := by
+      rw [<- small_final]
+      assumption
+    rw [<- hc']
+    assumption
+  }
+
