case_study/lean/Hammered.lean
@@ -1,0 +1,2 @@
+import Hammered.Big_Step
+import Hammered.Small_Step
