case_study/lean/Main.lean
@@ -1,5 +1,6 @@
 import Definitions
 import Base
+import Hammered
 
 def main : IO Unit :=
   IO.println s!"Hello, world!"
